Weidenbach_Book/Watched_Literals_List_Restart.thy
@@ -4030,6 +4030,24 @@ definition cdcl_twl_stgy_restart_abs_early_l :: "'v twl_st_l \<Rightarrow> 'v tw
     } else RETURN T
   }\<close>
 
+definition cdcl_twl_stgy_restart_abs_bounded_l :: "'v twl_st_l \<Rightarrow> (bool \<times> 'v twl_st_l) nres" where
+  \<open>cdcl_twl_stgy_restart_abs_bounded_l S\<^sub>0 =
+  do {
+    ebrk \<leftarrow> RES UNIV;
+    (_, brk, T, n) \<leftarrow> WHILE\<^sub>T\<^bsup>\<lambda>(ebrk, brk, T, n). cdcl_twl_stgy_restart_abs_l_inv S\<^sub>0 brk T n\<^esup>
+      (\<lambda>(ebrk, brk, _). \<not>brk \<and> \<not>ebrk)
+      (\<lambda>(_, brk, S, n).
+      do {
+        T \<leftarrow> unit_propagation_outer_loop_l S;
+        (brk, T) \<leftarrow> cdcl_twl_o_prog_l T;
+        (T, n) \<leftarrow> restart_abs_l T n brk;
+	ebrk \<leftarrow> RES UNIV;
+        RETURN (ebrk, brk, T, n)
+      })
+      (ebrk, False, S\<^sub>0, 0);
+    RETURN (brk, T)
+  }\<close>
+
 definition cdcl_twl_stgy_restart_prog_l :: "'v twl_st_l \<Rightarrow> 'v twl_st_l nres" where
   \<open>cdcl_twl_stgy_restart_prog_l S\<^sub>0 =
   do {
@@ -4258,7 +4276,119 @@ lemma (in twl_restart) cdcl_twl_stgy_restart_prog_l_cdcl_twl_stgy_restart_prog:
   apply simp
   done
 
-end
+
+definition cdcl_twl_stgy_restart_prog_bounded_l :: "'v twl_st_l \<Rightarrow> (bool \<times> 'v twl_st_l) nres" where
+  \<open>cdcl_twl_stgy_restart_prog_bounded_l S\<^sub>0 =
+  do {
+    ebrk \<leftarrow> RES UNIV;
+    (ebrk, brk, T, n) \<leftarrow> WHILE\<^sub>T\<^bsup>\<lambda>(ebrk, brk, T, n). cdcl_twl_stgy_restart_abs_l_inv S\<^sub>0 brk T n\<^esup>
+      (\<lambda>(ebrk, brk, _). \<not>brk \<and> \<not>ebrk)
+      (\<lambda>(ebrk, brk, S, n).
+      do {
+        T \<leftarrow> unit_propagation_outer_loop_l S;
+        (brk, T) \<leftarrow> cdcl_twl_o_prog_l T;
+        (T, n) \<leftarrow> restart_prog_l T n brk;
+	ebrk \<leftarrow> RES UNIV;
+        RETURN (ebrk, brk, T, n)
+      })
+      (ebrk, False, S\<^sub>0, 0);
+    RETURN (brk, T)
+  }\<close>
+
+
+lemma cdcl_twl_stgy_restart_abs_bounded_l_cdcl_twl_stgy_restart_abs_bounded_l:
+  \<open>(cdcl_twl_stgy_restart_abs_bounded_l, cdcl_twl_stgy_restart_prog_bounded) \<in>
+     {(S, S'). (S, S') \<in> twl_st_l None \<and> twl_list_invs S \<and>
+       clauses_to_update_l S  = {#}} \<rightarrow>\<^sub>f
+      \<langle>bool_rel \<times>\<^sub>r {(S, S'). (S, S') \<in> twl_st_l None \<and> twl_list_invs S}\<rangle> nres_rel\<close>
+  unfolding cdcl_twl_stgy_restart_abs_bounded_l_def cdcl_twl_stgy_restart_prog_bounded_def uncurry_def
+  apply (intro frefI nres_relI)
+  apply (refine_rcg
+	WHILEIT_refine[where R = \<open>{((ebrk :: bool, brk :: bool, S, n :: nat), (ebrk' :: bool, brk', S', n')).
+      (S, S') \<in> twl_st_l None \<and> twl_list_invs S \<and> brk = brk' \<and> n = n' \<and> ebrk = ebrk' \<and>
+        clauses_to_update_l S = {#}}\<close>]
+      unit_propagation_outer_loop_l_spec[THEN fref_to_Down]
+      cdcl_twl_o_prog_l_spec[THEN fref_to_Down]
+      restart_abs_l_restart_prog[THEN fref_to_Down_curry2])
+  subgoal by simp
+  subgoal for x y _ _ xa x' x1 x2 x1a x2a
+    unfolding cdcl_twl_stgy_restart_abs_l_inv_def
+    apply (rule_tac x=y in exI)
+    apply (rule_tac x=\<open>fst (snd (snd x'))\<close> in exI)
+    by auto
+  subgoal by fast
+  subgoal
+    unfolding cdcl_twl_stgy_restart_prog_inv_def
+      cdcl_twl_stgy_restart_abs_l_inv_def
+    apply (simp only: prod.case)
+    apply (normalize_goal)+
+    by (simp add: twl_st_l twl_st)
+  subgoal by (auto simp: twl_st_l twl_st)
+  subgoal by auto
+  subgoal by auto
+  subgoal by auto
+  done
+
+lemma cdcl_twl_stgy_restart_prog_bounded_l_cdcl_twl_stgy_restart_abs_bounded_l:
+  \<open>(cdcl_twl_stgy_restart_prog_bounded_l, cdcl_twl_stgy_restart_abs_bounded_l) \<in> {(S, S').
+   (S, S') \<in> Id \<and>  twl_list_invs S \<and>  clauses_to_update_l S = {#}} \<rightarrow>\<^sub>f \<langle>Id\<rangle> nres_rel\<close>
+   (is \<open>_ \<in> ?R \<rightarrow>\<^sub>f _\<close>)
+proof -
+  have [refine0]: \<open>((False, S, 0), (False, T , 0)) \<in> bool_rel \<times>\<^sub>r ?R \<times>\<^sub>r nat_rel\<close>
+    if \<open>(S, T) \<in> ?R\<close>
+    for S T
+    using that by auto
+  have [refine0]: \<open>unit_propagation_outer_loop_l x1c  \<le> \<Down> Id (unit_propagation_outer_loop_l x1a)\<close>
+    if \<open>(x1c, x1a) \<in> Id\<close>
+    for x1c x1a
+    using that by auto
+  have [refine0]: \<open>cdcl_twl_o_prog_l x1c  \<le> \<Down> Id (cdcl_twl_o_prog_l x1a)\<close>
+    if \<open>(x1c, x1a) \<in> Id\<close>
+    for x1c x1a
+    using that by auto
+  show ?thesis
+    unfolding cdcl_twl_stgy_restart_prog_bounded_l_def cdcl_twl_stgy_restart_prog_def uncurry_def
+      cdcl_twl_stgy_restart_abs_bounded_l_def
+    apply (intro frefI nres_relI)
+    apply (refine_rcg WHILEIT_refine[where R = \<open>{((brk :: bool, S, n :: nat), (brk', S', n')).
+        (S, S') \<in> Id \<and> brk = brk' \<and> n = n'}\<close>]
+	WHILEIT_refine[where R = \<open>{((ebrk :: bool, brk :: bool, S, n :: nat), (ebrk', brk', S', n')).
+        (S, S') \<in> Id \<and> brk = brk' \<and> n = n' \<and> ebrk = ebrk'}\<close> ]
+        unit_propagation_outer_loop_l_spec[THEN fref_to_Down]
+        cdcl_twl_o_prog_l_spec[THEN fref_to_Down]
+        restart_abs_l_restart_prog[THEN fref_to_Down_curry2]
+        restart_prog_l_restart_abs_l[THEN fref_to_Down_curry2])
+    subgoal by auto
+    subgoal for x y xa x' x1 x2 x1a x2a
+      by fastforce
+    subgoal by auto
+    subgoal
+      by (simp add: twl_st)
+    subgoal by (auto simp: twl_st)
+    subgoal
+       unfolding cdcl_twl_stgy_restart_prog_inv_def cdcl_twl_stgy_restart_abs_l_inv_def
+       by (auto simp: twl_st)
+    subgoal by auto
+    done
+qed
+
+
+
+lemma (in twl_restart) cdcl_twl_stgy_restart_prog_bounded_l_cdcl_twl_stgy_restart_prog_bounded:
+  \<open>(cdcl_twl_stgy_restart_prog_bounded_l, cdcl_twl_stgy_restart_prog_bounded)
+    \<in> {(S, S'). (S, S') \<in> twl_st_l None \<and> twl_list_invs S \<and> clauses_to_update_l S = {#}} \<rightarrow>\<^sub>f
+      \<langle>bool_rel \<times>\<^sub>r {(S, S'). (S, S') \<in> twl_st_l None \<and> twl_list_invs S}\<rangle>nres_rel\<close>
+  apply (intro frefI nres_relI)
+  apply (rule order_trans)
+  defer
+  apply (rule cdcl_twl_stgy_restart_abs_bounded_l_cdcl_twl_stgy_restart_abs_bounded_l[THEN fref_to_Down])
+    apply fast
+    apply assumption
+  apply (rule cdcl_twl_stgy_restart_prog_bounded_l_cdcl_twl_stgy_restart_abs_bounded_l[THEN fref_to_Down,
+    simplified])
+  apply simp
+  done
 
 end
 
+end
