Weidenbach_Book/Watched_Literals_Watch_List_Domain_Restart.thy
@@ -1772,6 +1772,48 @@ lemma cdcl_twl_stgy_restart_prog_early_wl_D_cdcl_twl_stgy_restart_prog_early_wl:
   subgoal by auto
   done
 
+definition cdcl_twl_stgy_restart_prog_bounded_wl_D
+  :: "nat twl_st_wl \<Rightarrow> (bool \<times> nat twl_st_wl) nres"
+where
+  \<open>cdcl_twl_stgy_restart_prog_bounded_wl_D S\<^sub>0 = do {
+    ebrk \<leftarrow> RES UNIV;
+    (ebrk, brk, T, n) \<leftarrow> WHILE\<^sub>T\<^bsup>\<lambda>(_, brk, T, n). cdcl_twl_stgy_restart_abs_wl_D_inv S\<^sub>0 brk T n\<^esup>
+      (\<lambda>(ebrk, brk, _). \<not>brk \<and> \<not>ebrk)
+      (\<lambda>(_, brk, S, n).
+      do {
+        T \<leftarrow> unit_propagation_outer_loop_wl_D S;
+        (brk, T) \<leftarrow> cdcl_twl_o_prog_wl_D T;
+        (T, n) \<leftarrow> restart_prog_wl_D T n brk;
+        ebrk \<leftarrow> RES UNIV;
+        RETURN (ebrk, brk, T, n)
+      })
+      (ebrk, False, S\<^sub>0::nat twl_st_wl, 0);
+    RETURN (brk, T)
+  }\<close>
+
+
+lemma cdcl_twl_stgy_restart_prog_bounded_wl_D_cdcl_twl_stgy_restart_prog_bounded_wl:
+  \<open>(cdcl_twl_stgy_restart_prog_bounded_wl_D, cdcl_twl_stgy_restart_prog_bounded_wl) \<in>
+     {(S, T). (S, T) \<in> Id \<and> literals_are_\<L>\<^sub>i\<^sub>n (all_atms_st S) S} \<rightarrow>\<^sub>f
+     \<langle>bool_rel \<times>\<^sub>r {(S, T). (S, T) \<in> Id \<and> literals_are_\<L>\<^sub>i\<^sub>n (all_atms_st S) S}\<rangle>nres_rel\<close>
+  unfolding uncurry_def cdcl_twl_stgy_restart_prog_bounded_wl_D_def
+    cdcl_twl_stgy_restart_prog_bounded_wl_def
+  apply (intro frefI nres_relI)
+  apply (refine_vcg
+      restart_prog_wl_D_restart_prog_wl[THEN fref_to_Down_curry2]
+      cdcl_twl_o_prog_wl_D_spec'[THEN fref_to_Down]
+      unit_propagation_outer_loop_wl_D_spec'[THEN fref_to_Down]
+      WHILEIT_refine[where R=\<open>bool_rel \<times>\<^sub>r bool_rel \<times>\<^sub>r {(S, T). (S, T) \<in> Id \<and>
+         literals_are_\<L>\<^sub>i\<^sub>n (all_atms_st S) S} \<times>\<^sub>r nat_rel\<close>])
+  subgoal by auto
+  subgoal unfolding  cdcl_twl_stgy_restart_abs_wl_D_inv_def by auto
+  subgoal by auto
+  subgoal by auto
+  subgoal by auto
+  subgoal by auto
+  subgoal by auto
+  subgoal by auto
+  done
 
 end
 
