Weidenbach_Book/Watched_Literals_Watch_List_Restart.thy
@@ -1228,8 +1228,61 @@ theorem cdcl_twl_stgy_restart_prog_early_wl_spec:
    (is \<open>?o \<in> ?A \<rightarrow> \<langle>?B\<rangle> nres_rel\<close>)
   using cdcl_twl_stgy_restart_prog_early_wl_cdcl_twl_stgy_restart_prog_early_l[where 'a='v]
   unfolding fref_param1 apply -
-  apply (match_spec; match_fun_rel+; (fast intro: nres_rel_mono)?)
-  by (metis (no_types, lifting) in_pair_collect_simp nres_rel_mono subrelI)
+  by (match_spec; match_fun_rel+; (fast intro: nres_rel_mono)?; match_fun_rel?)
+    auto
+
+definition (in twl_restart_ops) cdcl_twl_stgy_restart_prog_bounded_wl
+  :: \<open>'v twl_st_wl \<Rightarrow> (bool \<times> 'v twl_st_wl) nres\<close>
+where
+  \<open>cdcl_twl_stgy_restart_prog_bounded_wl (S\<^sub>0::'v twl_st_wl) = do {
+    ebrk \<leftarrow> RES UNIV;
+    (_, brk, T, n) \<leftarrow> WHILE\<^sub>T\<^bsup>\<lambda>(_, brk, T, n). cdcl_twl_stgy_restart_abs_wl_inv S\<^sub>0 brk T n\<^esup>
+      (\<lambda>(ebrk, brk, _). \<not>brk \<and> \<not>ebrk)
+      (\<lambda>(_, brk, S, n).
+      do {
+        T \<leftarrow> unit_propagation_outer_loop_wl S;
+        (brk, T) \<leftarrow> cdcl_twl_o_prog_wl T;
+        (T, n) \<leftarrow> restart_prog_wl T n brk;
+	ebrk \<leftarrow> RES UNIV;
+        RETURN (ebrk, brk, T, n)
+      })
+      (ebrk, False, S\<^sub>0::'v twl_st_wl, 0);
+    RETURN (brk, T)
+  }\<close>
+
+
+lemma cdcl_twl_stgy_restart_prog_bounded_wl_cdcl_twl_stgy_restart_prog_bounded_l:
+  \<open>(cdcl_twl_stgy_restart_prog_bounded_wl, cdcl_twl_stgy_restart_prog_bounded_l)
+    \<in> {(S, T).  (S, T) \<in> state_wl_l None \<and> correct_watching S} \<rightarrow>\<^sub>f
+      \<langle>bool_rel \<times>\<^sub>r {(S, T).  (S, T) \<in> state_wl_l None \<and> correct_watching S}\<rangle>nres_rel\<close>
+  (is \<open>_ \<in> ?R \<rightarrow>\<^sub>f \<langle>?S\<rangle>nres_rel\<close>)
+proof -
+  show ?thesis
+    unfolding cdcl_twl_stgy_restart_prog_bounded_wl_def cdcl_twl_stgy_restart_prog_bounded_l_def
+    apply (intro frefI nres_relI)
+    apply (refine_rcg
+        WHILEIT_refine[where R=\<open>bool_rel \<times>\<^sub>r bool_rel \<times>\<^sub>r ?R \<times>\<^sub>r nat_rel\<close>]
+      unit_propagation_outer_loop_wl_spec[THEN fref_to_Down]
+      cdcl_twl_full_restart_wl_prog_cdcl_twl_restart_l_prog[THEN fref_to_Down_curry2]
+      cdcl_twl_o_prog_wl_spec[THEN fref_to_Down])
+    subgoal by auto
+    subgoal unfolding cdcl_twl_stgy_restart_abs_wl_inv_def by fastforce
+    subgoal by auto
+    subgoal by (auto simp: correct_watching_correct_watching)
+    subgoal by auto
+    subgoal by auto
+    subgoal by auto
+    done
+qed
+
+theorem cdcl_twl_stgy_restart_prog_bounded_wl_spec:
+  \<open>(cdcl_twl_stgy_restart_prog_bounded_wl, cdcl_twl_stgy_restart_prog_bounded_l) \<in> {(S::'v twl_st_wl, S').
+       (S, S') \<in> state_wl_l None \<and> correct_watching S} \<rightarrow> \<langle>bool_rel \<times>\<^sub>r state_wl_l None\<rangle>nres_rel\<close>
+   (is \<open>?o \<in> ?A \<rightarrow> \<langle>?B\<rangle> nres_rel\<close>)
+  using cdcl_twl_stgy_restart_prog_bounded_wl_cdcl_twl_stgy_restart_prog_bounded_l[where 'a='v]
+  unfolding fref_param1 apply -
+  by (match_spec; match_fun_rel+; (fast intro: nres_rel_mono)?; match_fun_rel?)
+    auto
 
 end
 
